proof/CCP/Coercion.v
@@ -7,7 +7,17 @@ Require Import CCP.Types.
 Require Import CCP.Thinning.
 Require Import CCP.Substitution.
 
+v v v v v v v
+*************
+v v v v v v v
+Lemma refl_coerce : forall U, U >> U.
+Proof.
+  intros.
+  apply coerce_conv ; auto with coc core.
+Qed.
+^ ^ ^ ^ ^ ^ ^
 
+v v v v v v v
 Inductive coerce_in_env : env -> env -> Prop :=
 | coerce_env_hd : forall e t u,
   forall s, e |- t : (Srt s) -> e |- u : (Srt s) ->
@@ -31,6 +41,12 @@ elim H.
 do 4 intro.
 rewrite H0.
 inversion_clear H1.
+*************
+^ ^ ^ ^ ^ ^ ^
+Lemma coerce_conv_coerce : forall U U' V V', conv U U' -> conv V V' ->
+  U >> V -> U' >> V'.
+Proof.
+^ ^ ^ ^ ^ ^ ^
 intros.
 inversion_clear H1.
 right.
@@ -58,11 +74,18 @@ apply thinning_n_coerce with l; auto with coc.
 left.
 exists x; auto with coc core arith datatypes.
 
+v v v v v v v
 do 5 intro.
 elim H0.
 do 4 intro.
 rewrite H1.
 inversion_clear H2.
+*************
+v v v v v v v
+Lemma sym_coerce : forall U V, U >> V -> V >> U.
+^ ^ ^ ^ ^ ^ ^
+Proof.
+^ ^ ^ ^ ^ ^ ^
 intros.
 inversion_clear H2.
 left.
@@ -114,6 +137,7 @@ apply (H8 w).
 exists x; auto with coc core arith datatypes.
 Qed.
 
+v v v v v v v
 Lemma typ_conv_env :
   forall e t T, typ e t T -> 
   forall f, coerce_in_env e f -> 
@@ -127,7 +151,20 @@ induction IHt using typ_mut with
   forall f, coerce_in_env e f -> 
   wf f -> f |- T >> U) ; intros ;
 auto with coc core arith datatypes.
+*************
+v v v v v v v
+Lemma coerce_subst_rec : forall U V,  U >> V -> forall u v, conv u v -> forall n, subst_rec u U n >> subst_rec v V n.
+^ ^ ^ ^ ^ ^ ^
+Proof.
+v v v v v v v
+  induction 1 ; intros ; simpl.
+  apply coerce_conv ; auto with coc.
+ 
+ apply coerce_prod ; auto with coc.
+^ ^ ^ ^ ^ ^ ^
+^ ^ ^ ^ ^ ^ ^
 
+v v v v v v v
 elim conv_item with n T e f; auto with coc core arith datatypes; intros.
 repeat destruct H1.
 destruct H2.
@@ -135,13 +172,31 @@ destruct H2.
 destruct H3.
 destruct H3.
 apply type_conv with x x0 ; auto with coc core.
+*************
+v v v v v v v
+ apply coerce_sum ; auto with coc.
+^ ^ ^ ^ ^ ^ ^
+^ ^ ^ ^ ^ ^ ^
 
+v v v v v v v
 cut (wf (T :: f)); intros.
 apply type_abs with s1 s2; auto with coc core arith datatypes.
 apply wf_var with s1; auto with coc core arith datatypes.
+*************
+v v v v v v v
+ apply coerce_sub_l ; auto with coc.
+^ ^ ^ ^ ^ ^ ^
+^ ^ ^ ^ ^ ^ ^
 
+v v v v v v v
 apply type_app with V; auto with coc core arith datatypes.
+*************
+v v v v v v v
+ apply coerce_sub_r ; auto with coc.
+^ ^ ^ ^ ^ ^ ^
+^ ^ ^ ^ ^ ^ ^
 
+v v v v v v v
 cut (wf (U :: f)); intros.
 apply type_pair with s1 s2; auto with coc core arith datatypes.
 apply wf_var with s1 ; auto with coc core.
@@ -180,8 +235,14 @@ apply coerce_sum with s ;auto with coc core arith datatypes.
 apply wf_var with s ; auto with coc core arith datatypes.
 
 apply coerce_beta with B C s ; auto with coc core arith datatypes.
+*************
+v v v v v v v
+ apply coerce_trans with (subst_rec u B n) ; auto with coc.
+^ ^ ^ ^ ^ ^ ^
 Qed.
+^ ^ ^ ^ ^ ^ ^
 
+v v v v v v v
 Lemma coerce_conv_env :
   forall e T U, e |- T >> U -> 
   forall f, coerce_in_env e f -> 
@@ -253,22 +314,38 @@ Qed.
 Lemma subset_support_not_sort : forall e t T, e |- t : T -> 
   forall U P, t = Subset U P -> 
   forall s, ~ (conv U (Srt s)).
+*************
+v v v v v v v
+Lemma subst_coerce : forall U V, U >> V -> forall t, subst t U >> subst t V.
+^ ^ ^ ^ ^ ^ ^
 Proof.
   induction 1 ; intros ; try discriminate.
 
   red ; intros.
   injection H1.
   intros.
+v v v v v v v
   rewrite <- H4 in H2.
 Admitted.
+*************
+  unfold subst ; apply coerce_subst_rec ; auto with coc.
+Qed.
+^ ^ ^ ^ ^ ^ ^
+^ ^ ^ ^ ^ ^ ^
 
+v v v v v v v
 Require Import CCP.Generation.
 
 Lemma coerce_sort : forall e T U, e |- T >> U ->
   forall r, e |- T : (Srt r) -> e |- U : (Srt r) ->
   forall s,
   (conv T (Srt s) -> conv U (Srt s)) /\ (conv U (Srt s) -> conv T (Srt s)).
+*************
+v v v v v v v
+Lemma coerce_lift_rec : forall U V,  U >> V -> forall n k, lift_rec k U n >> lift_rec k V n.
+^ ^ ^ ^ ^ ^ ^
 Proof.
+v v v v v v v
   induction 1
  using coerce_mut with
   (P := fun e t T => fun H : typ e t T =>
@@ -279,17 +356,37 @@ Proof.
   forall s,
   (conv T (Srt s) -> conv U (Srt s)) /\ (conv U (Srt s) -> conv T (Srt s))) ; intros ;
 auto with coc core arith datatypes ; try discriminate.
+*************
+  induction 1 ; intros ; simpl.
+  apply coerce_conv ; auto with coc.
+ 
+ apply coerce_prod ; auto with coc.
+^ ^ ^ ^ ^ ^ ^
+^ ^ ^ ^ ^ ^ ^
 
+v v v v v v v
   injection H.
   intros.
   inversion H0.
   rewrite H1 ; auto.
+*************
+v v v v v v v
+ apply coerce_sum ; auto with coc.
+^ ^ ^ ^ ^ ^ ^
+^ ^ ^ ^ ^ ^ ^
 
+v v v v v v v
   destruct (typ_sort H2 (refl_equal (Srt prop))).
   rewrite H10 in H4.
   pose (typ_not_kind H4).
   elim n ; auto.
+*************
+v v v v v v v
+ apply coerce_sub_l ; auto with coc.
+^ ^ ^ ^ ^ ^ ^
+^ ^ ^ ^ ^ ^ ^
 
+v v v v v v v
   injection H.
   intros.
   case (typ_sort H0 (refl_equal (Srt set))).
@@ -298,8 +395,21 @@ auto with coc core arith datatypes ; try discriminate.
   auto with coc.
   
   inversion i.
+*************
+v v v v v v v
+ apply coerce_sub_r ; auto with coc.
+^ ^ ^ ^ ^ ^ ^
+^ ^ ^ ^ ^ ^ ^
 
+v v v v v v v
+*************
+v v v v v v v
+ apply coerce_trans with (lift_rec k B n) ; auto with coc.
+Qed.
+^ ^ ^ ^ ^ ^ ^
+^ ^ ^ ^ ^ ^ ^
 
+v v v v v v v
   induction H0.
 
   
@@ -358,6 +468,10 @@ auto with coc core arith datatypes ; try discriminate.
 Lemma coerce_sym : forall e T U, e |- T >> U ->
   forall s, e |- T : Srt s -> e |- U : Srt s -> 
   e |- U >> T.
+*************
+v v v v v v v
+Lemma lift_coerce : forall U V, U >> V -> forall n, lift n U >> lift n V.
+^ ^ ^ ^ ^ ^ ^
 Proof.
   intros e T U H ; induction H ; intros ; auto with coc core.
   
@@ -367,6 +481,7 @@ Proof.
   cut (coerce_in_env (A' :: G) (A :: G)).
   cut (coerce_in_env (A :: G) (A' :: G)).
   intros.
+v v v v v v v
   
   apply coerce_conv_env with (A' :: G) ; auto with coc core.
  
@@ -380,7 +495,18 @@ Proof.
   inversion H11.
   apply typ_conv_env with (A :: G) ; auto with coc core.
   apply wf_var with s ; auto with coc core.
+*************
+  unfold lift ; apply coerce_lift_rec ; auto with coc.
+^ ^ ^ ^ ^ ^ ^
+Qed.
+v v v v v v v
+^ ^ ^ ^ ^ ^ ^
 
+v v v v v v v
   apply coerce_env_
 
   
+*************
+Hint Resolve refl_coerce sym_coerce subst_coerce lift_coerce : coc.
+^ ^ ^ ^ ^ ^ ^
+^ ^ ^ ^ ^ ^ ^
