proof/CCP/Inversion.v
@@ -2,7 +2,9 @@ Require Import Termes.
 Require Import Reduction.
 Require Import Conv.
 Require Import LiftSubst.
+v v v v v v v
 Require Import Env.
+^ ^ ^ ^ ^ ^ ^
 Require Import CCP.Types.
 Require Import CCP.Coercion.
 Require Import CCP.Thinning.
@@ -11,12 +13,21 @@ Require Import CCP.Substitution.
 Implicit Types i k m n p : nat.
 Implicit Type s : sort.
 Implicit Types A B M N T t u v : term.
+v v v v v v v
 Implicit Types e f g : env.
+^ ^ ^ ^ ^ ^ ^
 
   Definition inv_type (P : Prop) e t T : Prop :=
     match t with
+v v v v v v v
     | Srt prop => coerce e T (Srt kind) -> P
     | Srt set => coerce e T (Srt kind) -> P
+*************
+v v v v v v v
+    | Srt prop => coerce T (Srt kind) -> P
+    | Srt set => coerce T (Srt kind) -> P
+^ ^ ^ ^ ^ ^ ^
+^ ^ ^ ^ ^ ^ ^
     | Srt kind => True
     | Ref n => forall x : term, item _ x e n -> coerce e T (lift (S n) x) -> P
     | Abs A M =>
@@ -33,12 +44,30 @@ Implicit Types e f g : env.
             typ e v (subst u V) -> T' = (Sum U V) -> coerce e T (Sum U V) -> P
     | Prod A B =>
         forall s1 s2,
+v v v v v v v
         typ e A (Srt s1) -> typ (A :: e) B (Srt s2) -> coerce e T (Srt s2) -> P
+*************
+v v v v v v v
+        typ e A (Srt s1) -> typ (A :: e) B (Srt s2) -> coerce T (Srt s2) -> P
+^ ^ ^ ^ ^ ^ ^
+^ ^ ^ ^ ^ ^ ^
     | Sum A B =>
         forall s1 s2,
+v v v v v v v
         typ e A (Srt s1) -> typ (A :: e) B (Srt s2) -> coerce e T (Srt s2) -> P
+*************
+v v v v v v v
+        typ e A (Srt s1) -> typ (A :: e) B (Srt s2) -> coerce T (Srt s2) -> P
+^ ^ ^ ^ ^ ^ ^
+^ ^ ^ ^ ^ ^ ^
     | Subset A B =>
+v v v v v v v
         typ e A (Srt set) -> typ (A :: e) B (Srt prop) -> coerce e T (Srt set) -> P
+*************
+v v v v v v v
+        typ e A (Srt set) -> typ (A :: e) B (Srt prop) -> coerce T (Srt set) -> P
+^ ^ ^ ^ ^ ^ ^
+^ ^ ^ ^ ^ ^ ^
     | Pi1 t =>
         forall U V,
         typ e t (Sum U V) -> coerce e T U -> P
@@ -66,9 +95,13 @@ case t; simpl in |- *; intros.
 generalize H0 ; clear H0.
 elim s; auto with coc core arith datatypes; intros.
 
+v v v v v v v
 apply H1 with x; auto with coc core arith datatypes.
+^ ^ ^ ^ ^ ^ ^
 
+v v v v v v v
 apply H1 with s1 s2 U0; auto with coc core arith datatypes.
+^ ^ ^ ^ ^ ^ ^
 
 apply H1 with Ur V0; auto with coc core arith datatypes.
 
@@ -85,11 +118,16 @@ apply H1 with U0 V0; auto with coc core arith datatypes.
 apply H1 with U0 s1 M s2; auto with coc core arith datatypes.
 
 intros.
+v v v v v v v
 induction H ; induction H0 ; auto with coc core.
 
 Admitted.
 (*pose coerce_beta.
+*************
+v v v v v v v
+^ ^ ^ ^ ^ ^ ^
 apply coerce_trans with V; auto with coc core arith datatypes.
+^ ^ ^ ^ ^ ^ ^
 Qed.
 *)
   Theorem typ_inversion :
@@ -119,7 +157,13 @@ apply H2 with U V; auto with coc core arith datatypes.
 apply H8 with U s1 M s2; auto with coc core arith datatypes.
 
 apply H1.
+v v v v v v v
 apply inv_type_coerce with V s; auto with coc core arith datatypes.
+*************
+v v v v v v v
+apply inv_type_coerce with V; auto with coc core arith datatypes.
+^ ^ ^ ^ ^ ^ ^
+^ ^ ^ ^ ^ ^ ^
 Qed.
 
 
@@ -129,13 +173,25 @@ apply typ_inversion with e (Srt kind) t; simpl in |- *;
  auto with coc core arith datatypes.
 Qed.
 
+v v v v v v v
   Lemma inv_typ_prop : forall e T, typ e (Srt prop) T -> coerce e T (Srt kind).
+*************
+v v v v v v v
+  Lemma inv_typ_prop : forall e T, typ e (Srt prop) T -> coerce T (Srt kind).
+^ ^ ^ ^ ^ ^ ^
+^ ^ ^ ^ ^ ^ ^
 intros.
 apply typ_inversion with e (Srt prop) T; simpl in |- *;
  auto with coc core arith datatypes.
 Qed.
 
+v v v v v v v
   Lemma inv_typ_set : forall e T, typ e (Srt set) T -> coerce e T (Srt kind).
+*************
+v v v v v v v
+  Lemma inv_typ_set : forall e T, typ e (Srt set) T -> coerce T (Srt kind).
+^ ^ ^ ^ ^ ^ ^
+^ ^ ^ ^ ^ ^ ^
 intros.
 apply typ_inversion with e (Srt set) T; simpl in |- *;
  auto with coc core arith datatypes.
@@ -144,7 +200,13 @@ Qed.
   Lemma inv_typ_ref :
    forall (P : Prop) e T n,
    typ e (Ref n) T ->
+v v v v v v v
    (forall U : term, item _ U e n -> coerce e T (lift (S n) U) -> P) -> P.
+*************
+v v v v v v v
+   (forall U : term, item _ U e n -> coerce T (lift (S n) U) -> P) -> P.
+^ ^ ^ ^ ^ ^ ^
+^ ^ ^ ^ ^ ^ ^
 intros.
 apply typ_inversion with e (Ref n) T; simpl in |- *; intros;
  auto with coc core arith datatypes.
@@ -156,7 +218,13 @@ Qed.
    typ e (Abs A M) U ->
    (forall s1 s2 T,
     typ e A (Srt s1) ->
+v v v v v v v
     typ (A :: e) M T -> typ (A :: e) T (Srt s2) -> coerce e (Prod A T) U -> P) ->
+*************
+v v v v v v v
+    typ (A :: e) M T -> typ (A :: e) T (Srt s2) -> coerce (Prod A T) U -> P) ->
+^ ^ ^ ^ ^ ^ ^
+^ ^ ^ ^ ^ ^ ^
    P.
 intros.
 apply typ_inversion with e (Abs A M) U; simpl in |- *;
@@ -168,7 +236,13 @@ Qed.
    forall (P : Prop) e u v T,
    typ e (App u v) T ->
    (forall V Ur : term,
+v v v v v v v
     typ e u (Prod V Ur) -> typ e v V -> coerce e T (subst v Ur) -> P) -> P.
+*************
+v v v v v v v
+    typ e u (Prod V Ur) -> typ e v V -> coerce T (subst v Ur) -> P) -> P.
+^ ^ ^ ^ ^ ^ ^
+^ ^ ^ ^ ^ ^ ^
 intros.
 apply typ_inversion with e (App u v) T; simpl in |- *;
  auto with coc core arith datatypes; intros.
@@ -181,7 +255,13 @@ Qed.
    (forall T U V : term, forall s1 s2,
      typ e U (Srt s1) ->
      typ e u U -> typ (U :: e) V (Srt s2) -> typ e v (subst u V) ->
+v v v v v v v
      T = (Sum U V) -> coerce e T' (Sum U V) -> P) -> P.
+*************
+v v v v v v v
+     T = (Sum U V) -> coerce T' (Sum U V) -> P) -> P.
+^ ^ ^ ^ ^ ^ ^
+^ ^ ^ ^ ^ ^ ^
 intros.
 apply typ_inversion with e (Pair T u v) T'; simpl in |- *;
  auto with coc core arith datatypes; intros.
@@ -192,7 +272,13 @@ Qed.
    forall (P : Prop) e T (U s : term),
    typ e (Prod T U) s ->
    (forall s1 s2,
+v v v v v v v
     typ e T (Srt s1) -> typ (T :: e) U (Srt s2) -> coerce e (Srt s2) s -> P) -> P.
+*************
+v v v v v v v
+    typ e T (Srt s1) -> typ (T :: e) U (Srt s2) -> coerce (Srt s2) s -> P) -> P.
+^ ^ ^ ^ ^ ^ ^
+^ ^ ^ ^ ^ ^ ^
 intros.
 apply typ_inversion with e (Prod T U) s; simpl in |- *;
  auto with coc core arith datatypes; intros.
@@ -203,7 +289,13 @@ Qed.
    forall (P : Prop) e T (U s : term),
    typ e (Sum T U) s ->
    (forall s1 s2,
+v v v v v v v
     typ e T (Srt s1) -> typ (T :: e) U (Srt s2) -> coerce e (Srt s2) s -> P) -> P.
+*************
+v v v v v v v
+    typ e T (Srt s1) -> typ (T :: e) U (Srt s2) -> coerce (Srt s2) s -> P) -> P.
+^ ^ ^ ^ ^ ^ ^
+^ ^ ^ ^ ^ ^ ^
 intros.
 apply typ_inversion with e (Sum T U) s; simpl in |- *;
  auto with coc core arith datatypes; intros.
@@ -213,7 +305,13 @@ Qed.
   Lemma inv_typ_subset :
    forall (P : Prop) e T (U s : term),
    typ e (Subset T U) s ->
+v v v v v v v
    (typ e T (Srt set) -> typ (T :: e) U (Srt prop) -> coerce e (Srt set) s -> P) -> P.
+*************
+v v v v v v v
+   (typ e T (Srt set) -> typ (T :: e) U (Srt prop) -> coerce (Srt set) s -> P) -> P.
+^ ^ ^ ^ ^ ^ ^
+^ ^ ^ ^ ^ ^ ^
 intros.
 apply typ_inversion with e (Subset T U) s; simpl in |- *;
  auto with coc core arith datatypes; intros.
@@ -222,7 +320,13 @@ Qed.
 Lemma inv_typ_pi1 : 
   forall (P : Prop) e t T,
    typ e (Pi1 t) T ->
+v v v v v v v
    (forall U V, typ e t (Sum U V) ->  coerce e U T -> P) -> P.
+*************
+v v v v v v v
+   (forall U V, typ e t (Sum U V) ->  coerce U T -> P) -> P.
+^ ^ ^ ^ ^ ^ ^
+^ ^ ^ ^ ^ ^ ^
 Proof.
 intros.
 apply typ_inversion with e (Pi1 t) T; simpl in |- *;
@@ -233,7 +337,13 @@ Qed.
 Lemma inv_typ_pi2 : 
   forall (P : Prop) e t T,
    typ e (Pi2 t) T ->
+v v v v v v v
    (forall U V, typ e t (Sum U V) ->  coerce e (subst (Pi1 t) V) T -> P) -> P.
+*************
+v v v v v v v
+   (forall U V, typ e t (Sum U V) ->  coerce (subst (Pi1 t) V) T -> P) -> P.
+^ ^ ^ ^ ^ ^ ^
+^ ^ ^ ^ ^ ^ ^
 Proof.
 intros.
 apply typ_inversion with e (Pi2 t) T; simpl in |- *;
@@ -248,7 +358,13 @@ Lemma inv_typ_let_in :
    forall s1, typ e V (Srt s1) ->
    forall T', typ (V :: e) t T' ->
    forall s2, typ (V :: e) T' (Srt s2) ->
+v v v v v v v
    coerce e (subst v T')  T -> P) -> P.
+*************
+v v v v v v v
+   coerce (subst v T')  T -> P) -> P.
+^ ^ ^ ^ ^ ^ ^
+^ ^ ^ ^ ^ ^ ^
 Proof.
 intros.
 apply typ_inversion with e (Let_in v t) T; simpl in |- *;
@@ -313,19 +429,35 @@ inversion_clear H2.
 Qed.
 
 Lemma type_pair_unique : forall e t T, typ e t T -> forall U V u v, t = (Pair (Sum U V) u v) ->
+v v v v v v v
    coerce e T (Sum U V).
+*************
+v v v v v v v
+   coerce T (Sum U V).
+^ ^ ^ ^ ^ ^ ^
+^ ^ ^ ^ ^ ^ ^
 Proof.
 intros ; induction H ; try discriminate.
 injection H0 ; intros.
 rewrite H6 ; rewrite H7.
+v v v v v v v
 apply refl_coerce.
+^ ^ ^ ^ ^ ^ ^
 pose (IHtyp1 H0).
+v v v v v v v
 apply coerce_trans with U0; auto with coc core arith datatypes.
+^ ^ ^ ^ ^ ^ ^
 Qed.
 
 Lemma type_pair_unique2 : forall e t T, typ e t T -> 
+v v v v v v v
    forall T' u v, t = (Pair T' u v) -> exists U,  exists  V, T' = Sum U V /\ 
+v v v v v v v
+   coerce T (Sum U V).
+^ ^ ^ ^ ^ ^ ^
+*************
    coerce e T (Sum U V).
+^ ^ ^ ^ ^ ^ ^
 Proof.
 intros ; induction H ; try discriminate.
 injection H0 ; intros.
@@ -337,5 +469,7 @@ induction H3.
 induction H3.
 exists x ; exists x0.
 split ; auto with coc.
+v v v v v v v
 apply coerce_trans with U; auto with coc core arith datatypes.
+^ ^ ^ ^ ^ ^ ^
 Qed.
